hlist_aux.v
@@ -1,0 +1,27 @@
+Require Export hybrid.tactics.
+Require Export Coq.Lists.List.
+Require Export Coq.Program.Program.
+
+Set Implicit Arguments.
+
+Section list_head.
+
+  Variable A : Type.
+
+  Program Definition head (l : list A) : l <> nil -> A :=
+    match l as l return l <> [] -> A with
+    | [] => fun H => !
+    | x::xs => fun _ => x
+    end.
+
+End list_head.
+
+Section hlists_def.
+
+  Context `{B : A -> Type}.
+
+  Inductive hlist (l : list A) : Type :=
+  | HNil : forall `{l = nil}, hlist l
+  | HCons : forall `{H : l <> nil}, B (head H) -> hlist (tail l) -> hlist l.
+
+End hlists_def.
